theories/main.v
@@ -4,4 +4,16 @@ Theorem main : Goal.
 Proof.
 Admitted.
 
+(*|
+
+And to prove we're not cheating:
+
+|*)
+
 Print Assumptions main.
+
+(*|
+
+The result follows from standard axioms.
+
+|*)
